common/LanguageInterface.v
@@ -10,7 +10,7 @@ Set Implicit Arguments.
 
 (** * Semantic interface of languages *)
 
-Definition query: Type := signature * list val * mem.
+Definition query: Type := list val * mem.
 Definition reply: Type := val * mem.
 
 
@@ -18,62 +18,14 @@ Definition reply: Type := val * mem.
 
 Record callconv :=
   mk_callconv {
-    world_def: Type;
-    match_senv_def:
-      world_def ->
-      Senv.t ->
-      Senv.t ->
-      Prop;
-    match_query_def:
-      world_def -> signature ->
-      list val -> mem ->
-      list val -> mem ->
-      Prop;
-    match_reply_def:
-      world_def -> signature ->
-      list val -> mem -> val -> mem ->
-      list val -> mem -> val -> mem ->
-      Prop;
+    world: Type;
+    match_senv:
+      world -> Senv.t -> Senv.t -> Prop;
+    match_query:
+      world -> query -> query -> Prop;
+    match_reply:
+      world -> query -> query -> reply -> reply -> Prop;
   }.
-
-Record world (cc: callconv) :=
-  mk_world {
-    cc_world :> world_def cc;
-    world_sg: signature;
-    world_sargs: list val;
-    world_smem: mem;
-    world_targs: list val;
-    world_tmem: mem;
-  }.
-
-Definition match_senv cc (w: world cc) (ge1 ge2: Senv.t): Prop :=
-  match_senv_def cc w ge1 ge2.
-
-Inductive match_query cc: world cc -> query -> query -> Prop :=
-  match_query_intro w sg vargs1 m1 vargs2 m2:
-    match_query_def cc w sg vargs1 m1 vargs2 m2 ->
-    match_query
-      (mk_world cc w sg vargs1 m1 vargs2 m2)
-      (sg, vargs1, m1)
-      (sg, vargs2, m2).
-
-Inductive match_reply cc: world cc -> reply -> reply -> Prop :=
-  match_reply_intro w sg vargs1 m1 vres1 m1' vargs2 m2 vres2 m2':
-    match_reply_def cc w sg vargs1 m1 vres1 m1' vargs2 m2 vres2 m2' ->
-    match_reply
-      (mk_world cc w sg vargs1 m1 vargs2 m2)
-      (vres1, m1')
-      (vres2, m2').
-
-Lemma match_query_injective cc (w: world cc) q q1 q2:
-  match_query w q q1 ->
-  match_query w q q2 ->
-  q1 = q2.
-Proof.
-  destruct 1.
-  inversion 1.
-  reflexivity.
-Qed.
 
 (** ** Expected properties of external call steps *)
 
@@ -95,8 +47,8 @@ Record extcall_step_valid sg (vargs: list val) m1 vres m2 :=
       Mem.unchanged_on (loc_not_writable m1) m1 m2;
   }.
 
-Definition extcall_valid (q: query) (r: reply) :=
-  let '(sg, vargs, m) := q in
+Definition extcall_valid sg (q: query) (r: reply) :=
+  let '(vargs, m) := q in
   let '(vres, m') := r in
   extcall_step_valid sg vargs m vres m'.
 
@@ -104,12 +56,10 @@ Definition extcall_valid (q: query) (r: reply) :=
 
 Definition cc_id :=
   {|
-    world_def := unit;
-    match_senv_def w := eq;
-    match_query_def w sg vargs1 m1 vargs2 m2 :=
-      vargs1 = vargs2 /\ m1 = m2;
-    match_reply_def w sg vargs1 m1 vres1 m1' vargs2 m2 vres2 m2' :=
-      vres1 = vres2 /\ m1' = m2';
+    world := unit;
+    match_senv w := eq;
+    match_query w := eq;
+    match_reply w q1 q2 := eq;
   |}.
 
 (** ** Extension passes *)
@@ -119,55 +69,47 @@ Definition loc_out_of_bounds (m: mem) (b: block) (ofs: Z) : Prop :=
 
 Definition cc_extends :=
   {|
-    world_def := unit;
-    match_senv_def w := eq;
-    match_query_def w sg vargs1 m1 vargs2 m2 :=
-      Val.lessdef_list vargs1 vargs2 /\
-      Mem.extends m1 m2;
-    match_reply_def w sg vargs1 m1 vres1 m1' vargs2 m2 vres2 m2' :=
-      Val.lessdef vres1 vres2 /\
-      Mem.extends m1' m2' /\
-      Mem.unchanged_on (loc_out_of_bounds m1) m2 m2';
+    world := unit;
+    match_senv w := eq;
+    match_query w :=
+      fun '(vargs1, m1) '(vargs2, m2) =>
+        Val.lessdef_list vargs1 vargs2 /\
+        Mem.extends m1 m2;
+    match_reply w :=
+      fun '(vargs1, m1) '(vargs2, m2) '(vres1, m1') '(vres2, m2') =>
+        Val.lessdef vres1 vres2 /\
+        Mem.extends m1' m2' /\
+        Mem.unchanged_on (loc_out_of_bounds m1) m2 m2';
   |}.
 
-Lemma match_query_extends w sg vargs1 m1 vargs2 m2:
-  match_query (cc := cc_extends) w (sg, vargs1, m1) (sg, vargs2, m2) ->
+Lemma match_query_extends w vargs1 m1 vargs2 m2:
+  match_query cc_extends w (vargs1, m1) (vargs2, m2) ->
   Mem.extends m1 m2 /\
-  Val.lessdef_list vargs1 vargs2 /\
-  w = mk_world cc_extends tt sg vargs1 m1 vargs2 m2.
+  Val.lessdef_list vargs1 vargs2.
 Proof.
   inversion 1; subst.
-  destruct H2, w0.
-  eauto.
-Qed.
-
-Lemma match_query_extends_intro sg vargs1 m1 vargs2 m2:
-  Mem.extends m1 m2 ->
-  Val.lessdef_list vargs1 vargs2 ->
-  match_query
-    (mk_world cc_extends tt sg vargs1 m1 vargs2 m2)
-    (sg, vargs1, m1)
-    (sg, vargs2, m2).
-Proof.
-  constructor.
-  simpl.
   tauto.
 Qed.
 
-Lemma match_reply_extends_intro sg vargs1 m1 vres1 m1' vargs2 m2 vres2 m2':
+Lemma match_query_extends_intro w vargs1 m1 vargs2 m2:
+  Mem.extends m1 m2 ->
+  Val.lessdef_list vargs1 vargs2 ->
+  match_query cc_extends w (vargs1, m1) (vargs2, m2).
+Proof.
+  constructor; eauto.
+Qed.
+
+Lemma match_reply_extends_intro w vargs1 m1 vres1 m1' vargs2 m2 vres2 m2':
   Val.lessdef vres1 vres2 ->
   Mem.extends m1' m2' ->
   Mem.unchanged_on (loc_out_of_bounds m1) m2 m2' ->
-  match_reply
-    (mk_world cc_extends tt sg vargs1 m1 vargs2 m2)
-    (vres1, m1')
-    (vres2, m2').
+  match_reply cc_extends w (vargs1, m1) (vargs2, m2) (vres1, m1') (vres2, m2').
 Proof.
-  intros Hvres Hm' Hm2.
   constructor; simpl; auto.
 Qed.
 
-Hint Resolve match_query_extends_intro match_reply_extends_intro.
+Hint Resolve match_query_extends_intro.
+Hint Resolve match_reply_extends_intro.
 
 (** ** Injection passes *)
 
@@ -197,80 +139,54 @@ Definition inject_separated (f f': meminj) (m1 m2: mem): Prop :=
 
 Definition cc_inject :=
   {|
-    world_def := meminj;
-    match_senv_def := symbols_inject;
-    match_query_def f sg vargs1 m1 vargs2 m2 :=
-      Val.inject_list f vargs1 vargs2 /\
-      Mem.inject f m1 m2;
-    match_reply_def f sg vargs1 m1 vres1 m1' vargs2 m2 vres2 m2' :=
-      exists f',
-        Val.inject f' vres1 vres2 /\
-        Mem.inject f' m1' m2' /\
-        Mem.unchanged_on (loc_unmapped f) m1 m1' /\
-        Mem.unchanged_on (loc_out_of_reach f m1) m2 m2' /\
-        inject_incr f f' /\
-        inject_separated f f' m1 m2;
+    world := meminj;
+    match_senv := symbols_inject;
+    match_query f :=
+      fun '(vargs1, m1) '(vargs2, m2) =>
+        Val.inject_list f vargs1 vargs2 /\
+        Mem.inject f m1 m2;
+    match_reply f :=
+      fun '(vargs1, m1) '(vargs2, m2) '(vres1, m1') '(vres2, m2') =>
+        exists f',
+          Val.inject f' vres1 vres2 /\
+          Mem.inject f' m1' m2' /\
+          Mem.unchanged_on (loc_unmapped f) m1 m1' /\
+          Mem.unchanged_on (loc_out_of_reach f m1) m2 m2' /\
+          inject_incr f f' /\
+          inject_separated f f' m1 m2;
   |}.
 
-Lemma match_query_inject w sg vargs1 m1 vargs2 m2:
-  match_query w (sg, vargs1, m1) (sg, vargs2, m2) ->
-  exists f,
-    Mem.inject f m1 m2 /\
-    Val.inject_list f vargs1 vargs2 /\
-    w = mk_world cc_inject f sg vargs1 m1 vargs2 m2.
+Lemma match_query_inject f vargs1 m1 vargs2 m2:
+  match_query cc_inject f (vargs1, m1) (vargs2, m2) ->
+  Mem.inject f m1 m2 /\
+  Val.inject_list f vargs1 vargs2.
 Proof.
-  inversion 1; subst.
-  simpl in *.
-  destruct H2.
-  eauto.
-Qed.
-
-Lemma match_query_inject_intro f sg vargs1 m1 vargs2 m2:
-  Val.inject_list f vargs1 vargs2 ->
-  Mem.inject f m1 m2 ->
-  match_query
-    (mk_world cc_inject f sg vargs1 m1 vargs2 m2)
-    (sg, vargs1, m1)
-    (sg, vargs2, m2).
-Proof.
-  constructor.
   simpl.
   tauto.
 Qed.
 
-Lemma match_reply_inject_intro f f' sg vargs1 m1 vres1 m1' vargs2 m2 vres2 m2':
+Lemma match_query_inject_intro f vargs1 m1 vargs2 m2:
+  Val.inject_list f vargs1 vargs2 ->
+  Mem.inject f m1 m2 ->
+  match_query cc_inject f (vargs1, m1) (vargs2, m2).
+Proof.
+  simpl.
+  tauto.
+Qed.
+
+Lemma match_reply_inject_intro f f' vargs1 m1 vres1 m1' vargs2 m2 vres2 m2':
   Mem.inject f' m1' m2' ->
   Val.inject f' vres1 vres2 ->
   Mem.unchanged_on (loc_unmapped f) m1 m1' ->
   Mem.unchanged_on (loc_out_of_reach f m1) m2 m2' ->
   inject_incr f f' ->
   inject_separated f f' m1 m2 ->
-  match_reply
-    (mk_world cc_inject f sg vargs1 m1 vargs2 m2)
-    (vres1, m1')
-    (vres2, m2').
+  match_reply cc_inject f (vargs1, m1) (vargs2, m2) (vres1, m1') (vres2, m2').
 Proof.
-  constructor; simpl; eauto 10.
+  simpl.
+  exists f'.
+  tauto.
 Qed.
-
-Lemma match_reply_inject_intro_same f sg vargs1 m1 vres1 vargs2 m2 vres2:
-  Mem.inject f m1 m2 ->
-  Val.inject f vres1 vres2 ->
-  match_reply
-    (mk_world cc_inject f sg vargs1 m1 vargs2 m2)
-    (vres1, m1)
-    (vres2, m2).
-Proof.
-  intros Hm Hvres.
-  constructor; simpl.
-  exists f; intuition.
-  intros b1 b2 delta Hb1 Hb1'.
-  congruence.
-Qed.
-
-Hint Resolve match_query_inject_intro.
-Hint Resolve match_reply_inject_intro.
-Hint Resolve match_reply_inject_intro_same.
 
 (** This is usedful as a hint to resolve the premices of
   [match_reply_inject_intro]. *)
@@ -282,3 +198,20 @@ Proof.
 Qed.
 
 Hint Resolve same_inject_separated.
+
+Lemma match_reply_inject_intro_same f vargs1 m1 vres1 vargs2 m2 vres2:
+  Mem.inject f m1 m2 ->
+  Val.inject f vres1 vres2 ->
+  match_reply cc_inject f (vargs1, m1) (vargs2, m2) (vres1, m1) (vres2, m2).
+Proof.
+  simpl.
+  exists f.
+  intuition.
+Qed.
+
+Hint Resolve match_query_inject_intro.
+Hint Resolve match_reply_inject_intro.
+Hint Resolve match_reply_inject_intro_same.
+
+Global Opaque match_query.
+Global Opaque match_reply.
